ztest.sml
@@ -1,0 +1,104 @@
+
+val resp_def = 
+ qdefine_psym("resp",[‘f:A->B’,‘r1:A~>A’,‘r2:B~>B’])
+ ‘!y z.Holds(r1,y,z) ==> Holds(r2,App(f:A->B,y),App(f,z))’
+ |> gen_all |> store_as "resp_def";
+
+
+
+
+val rext_ex = prove_store("rext_ex",
+e0
+(cheat)
+(form_goal
+ “!A B f:A->B r1:A~>A r2:B~>B.
+ ?e:Pow(A) ~> Pow(B).
+  !sa sb. Holds(e,sa,sb) <=> 
+   ?a b.sa = rsi(r1,a) & sb = rsi(r2,b) &
+    App(f,a) = b”));
+
+val rext_def = rext_ex |> spec_all 
+                       |> qSKOLEM "rext"
+                       [‘f’,‘r1’,‘r2’]
+                       |> gen_all |> store_as "rext_def";
+
+val main = prove_store("main",
+e0
+cheat
+(form_goal
+“!A B f:A->B r1:A~>A r2:B~>B
+ Q1 Q2 i1:Q1->Pow(A) i2:Q2->Pow(B). 
+ ER(r1) & ER(r2) & resp(f,r1,r2) &
+ (!sa. (?q1. sa = App(i1,q1)) <=> (?a. sa = rsi(r1,a))) & 
+ (!sb. (?q2. sb = App(i2,q2)) <=> (?b. sb = rsi(r2,b))) ==>
+ ?qf: Q1-> Q2.
+ !q1:mem(Q1). Holds(rext(f,r1,r2),App(i1,q1),App(i2 o qf,q1)) ”));
+
+(* product rel *)
+val prrel_ex = prove_store("prrel_ex",
+e0
+(cheat)
+(form_goal “!A r1:A~>A B r2:B~>B. ?r:A * B ~> A * B.
+ !a1 b1 a2 b2.Holds(r,Pair(a1,b1),Pair(a2,b2)) <=> 
+ Holds(r1,a1,a2) & Holds(r2,b1,b2)”));
+
+val prrel_def = prrel_ex |> spec_all |> qSKOLEM "prrel"
+[‘r1’,‘r2’] |> gen_all |> store_as "prrel_def";
+
+
+
+val main = prove_store("main",
+e0
+cheat
+(form_goal
+“!A B f:A->B r1:A~>A r2:B~>B
+ Q1 Q2 i1:Q1->Pow(A) i2:Q2->Pow(B). 
+ ER(r1) & ER(r2) & resp(f,r1,r2) &
+ (!sa. (?q1. sa = App(i1,q1)) <=> (?a. sa = rsi(r1,a))) & 
+ (!sb. (?q2. sb = App(i2,q2)) <=> (?b. sb = rsi(r2,b))) ==>
+ ?qf: Q1-> Q2.
+ !q1:mem(Q1). Holds(rext(f,r1,r2),App(i1,q1),App(i2 o qf,q1)) ”));
+
+(*
+
+Pow(A) * Pow(A) -> Pow(A * A) not have in general.
+
+ *)
+
+
+val ipow2_ex = prove_store("ipow2_ex",
+e0
+cheat
+(form_goal “!i1:Q1-> Pow(A) i2:Q2 -> Pow(B). 
+ ?i: Q1 * Q2 -> Pow(A * B).
+ !aq bq.
+  !a1 a2.IN(Pair(a1,a2),App(i,Pair(aq,bq))) <=> 
+         IN(a1,App(i1,aq)) & IN(a2,App(i2,bq))”));
+
+
+val ipow2_def = ipow2_ex |> spec_all 
+                         |> qSKOLEM "ipow2" [‘i1’,‘i2’]
+                         |> gen_all
+
+main |> qspecl [‘(N * N) * (N * N)’,‘N * N’,
+                ‘addf0’,
+                ‘prrel(ZR,ZR)’,‘ZR’,
+                ‘Z * Z’,‘Z’,
+                ‘ipow2(iZ,iZ)’,‘iZ’]
+
+
+
+
+
+
+“Rsi(prrel(ZR,ZR)) = a”
+(*lift_fun_rel*)
+val Lfr_def =
+    AX1 |> qspecl [‘Y’,‘Y’] |> uex2ex_rule 
+        |> fVar_sInst_th “P(y1:mem(Y),y2:mem(Y))”
+           “?x1 x2. y1 = App(enc1:X->Y,x1) &
+                    y2 = App(enc2,x2) & App(f,x1) = x2”
+        |> qSKOLEM "Lfr" [‘f’,‘enc’]
+        |> gen_all
+        |> store_as "Lfr_def";
+
